Probably found the most convenient form of BPC_CHANGE lemma

src/ocamlmm/OCamlToimm_s_prog_compilation.v
@@ -438,10 +438,10 @@ Section OCaml_IMM_Correspondence.
     sto.(ectrl) = bsti.(bectrl) /\
     sto.(eindex) = bsti.(beindex).
 
-
   Definition omm_block_step (tid : thread_id) (bst1 bst2: block_state) :=
-    exists block, block_step_helper block tid bst1 bst2 /\
-             exists instr, is_instruction_compiled instr block. 
+    ⟪ BLOCK_STEP: exists block, block_step_helper block tid bst1 bst2 ⟫ /\
+    ⟪ BINSTRS_SAME: binstrs bst1 = binstrs bst2 ⟫ /\
+    ⟪ COMPILED: exists PO, is_thread_block_compiled PO (binstrs bst1) ⟫. 
   
   Lemma block_step_nonterminal bst bst' tid
         (OSEQ_STEP: block_step tid bst bst'):
@@ -454,9 +454,9 @@ Section OCaml_IMM_Correspondence.
     intuition. congruence.
   Qed.
 
-  Lemma bs_extract bst bst' tid (OSEQ_STEP: omm_block_step tid bst bst'):
+  Lemma bs_extract bst bst' tid (OMM_BLOCK_STEP: omm_block_step tid bst bst'):
     block_step tid bst bst'.
-  Proof. do 2 (red in OSEQ_STEP; desc). vauto. Qed.
+  Proof. red in OMM_BLOCK_STEP; desc. red in BLOCK_STEP. desc. vauto. Qed.
 
   Definition sublist {A: Type} (l: list A) (start len: nat) := firstn len (skipn start l).  
     
@@ -471,135 +471,79 @@ Section OCaml_IMM_Correspondence.
     rewrite H1. auto. 
   Qed.
 
-  Lemma BPC_CHANGE_foobar bst bst' tid
-        (OMM_BLOCK_STEP: omm_block_step tid bst bst')
-        (COMP: exists PO, is_thread_block_compiled PO (binstrs bst)):
-    bpc bst' = bpc bst + 1 \/ exists cond adr, Some [Instr.ifgoto cond adr] = nth_error (binstrs bst) (bpc bst).
+  Lemma BPC_CHANGE bst bst' tid (OMM_BLOCK_STEP: omm_block_step tid bst bst')
+        block (BLOCK: Some block = nth_error (binstrs bst) (bpc bst))
+        BPI0 block0 (CORR: block_corrected BPI0 block0 block):
+    bpc bst' =
+    match block, block0 with
+    | [Instr.ifgoto cond _], [Instr.ifgoto _ addr0]
+      => if Const.eq_dec (RegFile.eval_expr (bregf bst) cond) 0
+        then bpc bst + 1 else addr0
+    | _, _  => bpc bst + 1
+    end. 
+  Proof. Admitted. 
+  
+  (* (OMM_BLOCK_STEP: omm_block_step tid bst bst'): *)
+  Lemma ___BPC_CHANGE___ bst bst' tid
+        (BLOCK_STEP: exists block : list Instr.t, block_step_helper block tid bst bst')
+        (BINSTRS_SAME: binstrs bst = binstrs bst')
+        PO (COMPILED: is_thread_block_compiled PO (binstrs bst))
+        oinstr (OINSTR: Some oinstr = nth_error PO (bpc bst)):
+    match oinstr with
+    | Instr.ifgoto cond addr0 =>
+      bpc bst' = if Const.eq_dec (RegFile.eval_expr (bregf bst) cond) 0
+                 then bpc bst + 1
+                 else length (flatten (firstn addr0 (binstrs bst)))
+    | _ => bpc bst' = bpc bst + 1
+    end. 
+    (* bpc bst' = bpc bst + 1 \/ *)
+    (* (exists cond addr0, Some (Instr.ifgoto cond addr0) = nth_error PO (bpc bst) /\ *)
+    (*                ).  *)
   Proof.
-    red in OMM_BLOCK_STEP. desc. red in OMM_BLOCK_STEP. desc.
-    assert ((exists (cond : Instr.expr) (adr : nat),
-                block = [Instr.ifgoto cond adr])
-            \/ (forall (cond : Instr.expr) (adr : nat), ~ In (Instr.ifgoto cond adr) block)) as BLOCK_CONTENT.
-    { admit. }
-    (* remember (bst2st bst) as st. remember (bst2st bst') as st'.  *)
-    assert (block = sublist (instrs (bst2st bst)) (pc (bst2st bst)) (length block)).
-    { admit. }
-    destruct BLOCK_CONTENT.
-    { right. desc. exists cond. exists adr. congruence. }
-    left.
-    assert (pc (bst2st bst') = pc (bst2st bst) + length block) by admit.
-    unfold bst2st in H1. simpl in H1.
-    replace (binstrs bst') with (binstrs bst) in * by admit.
-    assert (length block > 0) as LENB. 
-    { inversion OMM_BLOCK_STEP0; vauto. }
-    assert (bpc bst' <= bpc bst \/ exists d, bpc bst' = bpc bst + S d) by admit.
-    desf. 
-    { assert (length (flatten (firstn (bpc bst') (binstrs bst)))
-              <= length (flatten (firstn (bpc bst) (binstrs bst)))).
-      { admit. }
-      omega. }
-    { destruct d; auto.
-      exfalso. 
-      rewrite H2 in *.
-      replace (bpc bst + S (S d)) with ((bpc bst + 1) + (d + 1)) in H1 by omega. 
-      replace (binstrs bst) with (firstn (bpc bst + 1) (binstrs bst) ++ skipn (bpc bst + 1) (binstrs bst)) in H1 at 1.
-      2: { apply firstn_skipn. }
-      replace (bpc bst + 1) with (length (firstn (bpc bst + 1) (binstrs bst))) in H1 at 1.
-      2: { apply firstn_length_le.
-           rewrite Nat.add_1_r. apply lt_le_S.
-           apply nth_error_Some. congruence. }
-      rewrite firstn_app_2 in H1.
-      rewrite (first_end _ _ AT_BLOCK) in H1.
-      rewrite !flatten_app, !app_length in H1. simpl in H1.
-      rewrite <- app_nil_end in H1.
-      assert (length (flatten (firstn (d + 1) (skipn (bpc bst + 1) (binstrs bst)))) = 0).
-      { omega. }
-      apply length_zero_iff_nil in H3.
-      assert (firstn (d + 1) (skipn (bpc bst + 1) (binstrs bst)) = []).
-      { destruct (firstn (d + 1) (skipn (bpc bst + 1) (binstrs bst))); auto.
-        admit. }
+    (* red in OMM_BLOCK_STEP. desc. red in BLOCK_STEP. desc. *)
+    (* assert ((exists (cond : Instr.expr) (adr : nat), *)
+    (*             block = [Instr.ifgoto cond adr]) *)
+    (*         \/ (forall (cond : Instr.expr) (adr : nat), ~ In (Instr.ifgoto cond adr) block)) as BLOCK_CONTENT. *)
+    (* { admit. } *)
+    (* assert (block = sublist (instrs (bst2st bst)) (pc (bst2st bst)) (length block)) as BLOCK_SPAN.  *)
+    (* { simpl. admit. } *)
+    (* destruct BLOCK_CONTENT. *)
+    (* { right. desc. exists cond. exists adr. congruence. } *)
+    (* assert (pc (bst2st bst') = pc (bst2st bst) + length block) as PC_ADVANCE. *)
+    (* { simpl. admit. } *)
+    (* unfold bst2st in PC_ADVANCE. simpl in PC_ADVANCE. *)
+    (* rewrite <- BINSTRS_SAME in *.  *)
+    (* assert (length block > 0) as LENB.  *)
+    (* { admit. } *)
+    (* assert (bpc bst' <= bpc bst \/ exists d, bpc bst' = bpc bst + S d) as BPC'.  *)
+    (* { destruct (le_dec (bpc bst') (bpc bst)); vauto. *)
+    (*   right. apply not_le in n. admit. } *)
+    (* desf.  *)
+    (* { assert (length (flatten (firstn (bpc bst') (binstrs bst))) *)
+    (*           <= length (flatten (firstn (bpc bst) (binstrs bst)))). *)
+    (*   { admit. } *)
+    (*   omega. } *)
+    (* { destruct d; auto. *)
+    (*   exfalso.  *)
+    (*   rewrite H2 in *. *)
+    (*   replace (bpc bst + S (S d)) with ((bpc bst + 1) + (d + 1)) in H1 by omega.  *)
+    (*   replace (binstrs bst) with (firstn (bpc bst + 1) (binstrs bst) ++ skipn (bpc bst + 1) (binstrs bst)) in H1 at 1. *)
+    (*   2: { apply firstn_skipn. } *)
+    (*   replace (bpc bst + 1) with (length (firstn (bpc bst + 1) (binstrs bst))) in H1 at 1. *)
+    (*   2: { apply firstn_length_le. *)
+    (*        rewrite Nat.add_1_r. apply lt_le_S. *)
+    (*        apply nth_error_Some. congruence. } *)
+    (*   rewrite firstn_app_2 in H1. *)
+    (*   rewrite (first_end _ _ AT_BLOCK) in H1. *)
+    (*   rewrite !flatten_app, !app_length in H1. simpl in H1. *)
+    (*   rewrite <- app_nil_end in H1. *)
+    (*   assert (length (flatten (firstn (d + 1) (skipn (bpc bst + 1) (binstrs bst)))) = 0). *)
+    (*   { omega. } *)
+    (*   apply length_zero_iff_nil in H3. *)
+    (*   assert (firstn (d + 1) (skipn (bpc bst + 1) (binstrs bst)) = []). *)
+    (*   { destruct (firstn (d + 1) (skipn (bpc bst + 1) (binstrs bst))); auto. *)
+    (*     admit. } *)
   Admitted. 
       
-      (* do 2 rewrite <- Nat.add_1_r, Const.add_assoc in H1. *)
-      (* assert (exists block', Some block' = nth_error (binstrs bst) (bpc bst) *)
-  (*   dest *)
-
-      (* foobar.  *)
-    (* inversion OMM_BLOCK_STEP0. *)
-      
-  (* Qed. *)
-
-  (* Lemma BPC_CHANGE_foobar2 bst bst' tid (OMM_BLOCK_STEP: omm_block_step tid bst bst') (COMP: exists PO, is_thread_block_compiled PO (binstrs bst)): *)
-  (*   bpc bst' = bpc bst + 1 \/ exists cond adr, Some [Instr.ifgoto cond adr] = nth_error (binstrs bst) (bpc bst). *)
-  (* Proof. *)
-  (*   red in OMM_BLOCK_STEP. desc. *)
-  (*   assert (binstrs bst = binstrs bst') as BINSTRS_SAME. *)
-  (*   { eapply (@SAME_BINSTRS _ _ tid). red. eauto. } *)
-  (*   red in OMM_BLOCK_STEP. desc. *)
-  (*   inversion OMM_BLOCK_STEP0. *)
-  (*   - left. subst. simpl in *. apply (same_relation_exp (seq_id_l (step tid))) in BLOCK_STEP. *)
-  (*     assert (Some ld = nth_error PO (bpc bst)). *)
-  (*     { assert (exists instr, Some instr = nth_error PO (bpc bst)). *)
-  (*       { apply OPT_VAL. apply nth_error_Some. *)
-  (*         rewrite (compilation_same_length COMP). *)
-  (*         apply nth_error_Some. eapply OPT_VAL. eauto. } *)
-  (*       desc. pose proof (every_instruction_compiled COMP _ H AT_BLOCK). *)
-  (*       inversion H0. vauto. } *)
-  (*     do 2 (red in BLOCK_STEP; desc). *)
-  (*     replace instr with ld in *. *)
-  (*     2: { foobar.  *)
-  (*     assert (AT_PC: Some ld = nth_error (instrs (bst2st bst)) (pc (bst2st bst))). *)
-  (*     {  *)
-  (*       apply eq_trans with (y := nth_error [ld] 0); auto. *)
-  (*       rewrite <- (NPeano.Nat.add_0_r (pc (bst2st bst))). *)
-  (*       eapply sublist_items; eauto. } *)
-  (*     inversion ISTEP0; rewrite <- AT_PC in ISTEP; inversion ISTEP; rewrite II in H2; subst ld. *)
-  (*     all: try discriminate H2. *)
-  (*     subst. unfold bst2st in UPC. simpl in UPC. *)
-  (* Admitted. *)
-
-  Lemma BPC_CHANGE bst bst' tid (OMM_BLOCK_STEP: omm_block_step tid bst bst'):
-    bpc bst' = bpc bst + 1 \/ exists cond adr, Some [Instr.ifgoto cond adr] = nth_error (binstrs bst) (bpc bst).
-  Proof.
-    red in OMM_BLOCK_STEP. desc. red in OMM_BLOCK_STEP. desc.
-    assert ((exists (cond : Instr.expr) (adr : nat),
-                block = [Instr.ifgoto cond adr])
-            \/ (forall (cond : Instr.expr) (adr : nat), ~ In (Instr.ifgoto cond adr) block)) as BLOCK_CONTENT.
-    { admit. }
-    destruct BLOCK_CONTENT.
-    { right. desc. exists cond. exists adr. congruence. }
-    left.
-    remember (bst2st bst) as st. remember (bst2st bst') as st'.
-    assert (pc st = length (flatten (firstn (bpc bst) (binstrs bst)))) by vauto. 
-    assert (pc st' = length (flatten (firstn (bpc bst') (binstrs bst)))) by admit.
-    assert (pc st' = pc st + length block) by admit.
-    rewrite H2 in H1. rewrite Heqst in H1. unfold bst2st in H1. simpl in H1.
-    rewrite <- app_length in H1.
-    replace (flatten (firstn (bpc bst) (binstrs bst)) ++ block) with (flatten (firstn (bpc bst) (binstrs bst) ++ [block])) in H1. 
-    2: { rewrite flatten_app. simpl. rewrite app_nil_r. auto. }
-    rewrite <- first_end in H1; auto.
-    assert (bpc bst' < bpc bst + 1 \/ bpc bst' = bpc bst + 1 \/ bpc bst' > bpc bst + 1) by omega. 
-    destruct H3 as [BPC | [BPC | BPC]]; auto; exfalso. 
-    {
-      (* set (strict_prefix_alt := fun {A: Type} (l1 l2: list A) => exists x l', l2 = l1 ++ x :: l'). *)
-      (* assert (strict_prefix_alt _ (firstn (bpc bst') (binstrs bst)) (firstn (bpc bst + 1) (binstrs bst))) by admit. *)
-      (* red in H4. desc. rewrite H4, flatten_app, app_length in H1. *)
-      (* simpl in H1. rewrite app_length in H1. *)
-      (* assert (length x > 0). *)
-      (* {  *)
-      (* assert (length (flatten l') = 0) by omega. *)
-      (* apply length_zero_iff_nil in H5. *)
-      admit. }
-
-    (* foobar. *)
-    
-    (* destruct H0. *)
-    (* { admit. } *)
-    (* desc. cut (d = 1); [ins; vauto|].   *)
-    (* unfold bst2st in BLOCK_STEP. rewrite H0 in *. simpl in *.  *)
-    (* assert (block = sublist (instrs (bst2st bst)) (pc (bst2st bst)) (length block)). *)
-    (* { admit. } *)
-    
-  Admitted. 
 
 End OCaml_IMM_Correspondence. 
